

MAT 120

DIFFERENTIAL EQN (DE)

Homogeneous Linear Eqn
with constant coefficients

Consider the n^{th} order DE below:

$$a_n y^{(n)} + a_{n-1} y^{(n-1)} + a_{n-2} y^{(n-2)} + \dots + a_2 y'' + a_1 y' + a_0 y = g(x) \quad \text{--- (i)}$$

if $g(x) = 0$ then (i) is a homogeneous DE

if $g(x) \neq 0$ then (i) is a non-homogeneous DE

Consider

$$a_n y^{(n)} + a_{n-1} y^{(n-1)} + \dots + a_2 y'' + a_1 y' + a_0 y = 0 \quad \text{--- (ii)}$$

(homogeneous DE)

Recall 1st order DE

$$a_1 y' + P(x)y = f(x) \quad \text{--- (iii)}$$

if (iii) is homogeneous DE

$$\text{then } a_1 y' + P(x)y = 0$$

Replace $a_1 = a$ & $P(x) = b$

$$\text{Now we have } ay' + by = 0$$

$$\frac{ay'}{a} + \frac{b}{a}y = 0$$

$$y' + \frac{b}{a}y = 0$$

$$\text{(iv)} \rightarrow y' + (m)y = 0 \quad \left\{ \begin{array}{l} \text{let } \frac{b}{a} = m \\ \text{Relabel constant} \end{array} \right\}$$

$$\text{I.F. } e^{\int P(x)dx} = e^{\int m dx} = e^{mx}$$

$$e^{mx} [y' + my] = e^{mx} (0) \quad \text{multiply (iv) with I.F.}$$

$$\int e^{mx} [y' + my] = \int 0 dx$$

$$ye^{mx} = C$$

$$y = Ce^{-mx}$$

$$y = e^{mx} \quad \text{--- (1)}$$

Relabel constants:
Consider $C=1$, $-m = +m$
Replace

∴ we found $y = e^{mx}$

$$\therefore y' = m e^{mx}$$

$$y'' = m^2 e^{mx}$$

$$y''' = m^3 e^{mx}$$

⋮

$$y^{(n-1)} = m^{n-1} e^{mx}$$

$$y^{(n)} = m^n e^{mx}$$

Substitute $y, y', y'', \dots, y^{(n)}$ into (i)

$$a_n m^n e^{mx} + a_{n-1} m^{n-1} e^{mx} + \dots + a_2 m^2 e^{mx} + a_1 m e^{mx} + a_0 e^{mx} = 0$$

(v)

eqn (v) may have distinct roots, repeating roots or complex roots.

Note eqn (v) is known as Auxiliary Equation.

Roots

Consider the following quadratic eqns:

(a) $2m^2 - 5m - 3 = 0$

$$\Rightarrow (2m+1)(m-3) = 0$$

$$\Rightarrow 2m+1 = 0 ; m-3 = 0$$

$$\Rightarrow m_1 = -\frac{1}{2}, m_2 = 3$$

here the solutions m_1, m_2 are distinct roots

(b) $m^2 - 10m + 25 = 0$

$$\Rightarrow (m-5)^2 = 0$$

$$\Rightarrow (m-5)(m-5) = 0$$

$$\Rightarrow m_1 = 5, m_2 = 5$$

here the solutions m_1, m_2 are repeating roots

Considering (a)

$$2m^2 - 5m - 3 = 0 \text{ — Auxiliary eqn (a)}$$

$$m_1 = -\frac{1}{2}, m_2 = 3$$

∴ the solutions are unique

∴ the solution of Auxiliary eqn (a) can be written as

$$y = c_1 e^{m_1 x} + c_2 e^{m_2 x}$$

$$= c_1 e^{-\frac{1}{2}x} + c_2 e^{3x}$$

$$= c_1 f_1(x) + c_2 f_2(x) \quad [\text{observe } f_1(x) \text{ \& } f_2(x) \text{ are independent}]$$

Considering (b)

$$m^2 - 10m + 25 = 0 \text{ — Auxiliary eqn (b)}$$

$$m_1 = 5, m_2 = 5$$

∴ the solutions are repeating

∴ the solution of Auxiliary eqn (b) can be written as

$$y = c_1 e^{m_1 x} + c_2 x e^{m_2 x}$$

$$= c_1 e^{5x} + c_2 x e^{5x}$$

$$= c_1 f_1(x) + c_2 f_2(x) \quad [\text{observe } f_1(x) \text{ \& } f_2(x) \text{ are}$$

now independent since

we introduced x along with

c_2 , otherwise the solution

will look like $\underbrace{c_1 e^{5x} + c_2 e^{5x}}_{\text{linearly dependent}}$

But we are looking forward to the independent set of solutions hence introduced x with c_2 .

Going back to eqn (V)

→ if the roots are non repeating : $m_1 \neq m_2 \neq m_3 \dots \neq m_n$

then solution of (V) will be:

$$y = c_1 e^{m_1 x} + c_2 e^{m_2 x} + \dots + c_n e^{m_n x}$$

→ If the roots are repeating : $m_1 = m_2 = m_3 \dots = m_n$

then the solution of (V) will be:

$$y = c_1 e^{m_1 x} + c_2 x e^{m_2 x} + c_3 x^2 e^{m_3 x} + c_4 x^3 e^{m_4 x} + \dots \\ \dots + c_n x^{n-1} e^{m_n x}$$

→ if the roots are complex numbers:

$$m = a \pm bi \Rightarrow m_1 = a + bi \\ m_2 = a - bi$$

then the solution of (V) will be:

$$y = c_1 e^{ax} \cos bx + c_2 e^{ax} \sin bx$$

Exercise

Find the General Solution of the given 2nd order differential eqn:

① $3y'' + 2y' + y = 0$ — (i)
substitute $y = e^{mx}$, $y' = m e^{mx}$, $y'' = m^2 e^{mx}$ into (i)

$$3m^2 e^{mx} + 2m e^{mx} + e^{mx} = 0$$

$$3m^2 + 2m + 1 = 0 \quad (\div \text{ by } e^{mx})$$

$$m = \frac{-2 \pm \sqrt{4 - 12}}{6}$$

$$= \frac{-2 \pm \sqrt{-8}}{6} = \frac{-2 \pm i2\sqrt{2}}{6} = \frac{-1 \pm i\sqrt{2}}{3} = -\frac{1}{3} \pm \frac{i\sqrt{2}}{3}$$

$$\therefore y = c_1 e^{-\frac{1}{3}x} \cos\left(\frac{\sqrt{2}}{3}x\right) + c_2 e^{-\frac{1}{3}x} \sin\left(\frac{\sqrt{2}}{3}x\right)$$

② $y'' - 3y' + 2y = 0$ — (i)

Substitute $y = e^{mx}$, $y' = me^{mx}$, $y'' = m^2 e^{mx}$ into (i)

$$m^2 e^{mx} - 3me^{mx} + 2e^{mx} = 0$$

$$m^2 - 3m + 2 = 0 \quad (\div \text{ by } e^{mx})$$

$$m^2 - 2m - m + 2 = 0$$

$$(m-2)(m-1) = 0$$

$$m_1 = 2, \quad m_2 = 1$$

$$\therefore y = c_1 e^{2x} + c_2 e^x$$

③ $y'' + 8y' + 16y = 0$ — (i)

Substitute $y = e^{mx}$, $y' = me^{mx}$, $y'' = m^2 e^{mx}$ into (i)

$$m^2 e^{mx} + 8me^{mx} + 16e^{mx} = 0$$

$$m^2 + 8m + 16 = 0 \quad (\div \text{ by } e^{mx})$$

$$m^2 + 2 \cdot m \cdot 4 + 4^2 = 0$$

$$(m+4)^2 = 0$$

$$(m+4)(m+4) = 0 \Rightarrow m_1 = m_2 = -4$$

$$\therefore y = c_1 e^{-4x} + c_2 x e^{-4x}$$

Find the General solution of higher order DE:

④ $16 \frac{d^4 y}{dx^4} + 24 \frac{d^2 y}{dx^2} + 9y = 0$ — (i)

Substitute $y = e^{mx}$, $y'' = m^2 e^{mx}$, $y^{(4)} = m^4 e^{mx}$ into (i)

$$16m^4 e^{mx} + 24m^2 e^{mx} + 9e^{mx} = 0$$

$$16m^4 + 24m^2 + 9 = 0$$

$$(4m^2)^2 + 2 \cdot 4m^2 \cdot 3 + 3^2 = 0 \Rightarrow (4m^2 + 3)^2 = 0$$

$$\Rightarrow (4m^2 + 3)(4m^2 + 3) = 0$$

$$4m^2 + 3 = 0$$

$$m_1 = m_2 = \pm \sqrt{\frac{-3}{4}}$$

$$= \pm i \frac{\sqrt{3}}{2}$$

$$= 0 \pm i\sqrt{3}/2$$

$$4m^2 + 3 = 0$$

$$m_3 = m_4 = \pm \sqrt{\frac{-3}{4}}$$

$$= \pm i \frac{\sqrt{3}}{2}$$

$$= 0 \pm i\sqrt{3}/2$$

m_3, m_4 are repeating roots of m_1, m_2

$$\therefore y = c_1 e^{0x} \cos\left(\frac{\sqrt{3}}{2}x\right) + c_2 e^{0x} \sin\left(\frac{\sqrt{3}}{2}x\right) + c_3 x e^{0x} \cos\left(\frac{\sqrt{3}}{2}x\right) + c_4 x e^{0x} \sin\left(\frac{\sqrt{3}}{2}x\right)$$

$$= c_1 \cos\left(\frac{\sqrt{3}}{2}x\right) + c_2 \sin\left(\frac{\sqrt{3}}{2}x\right) + c_3 x \cos\left(\frac{\sqrt{3}}{2}x\right) + c_4 x \sin\left(\frac{\sqrt{3}}{2}x\right)$$

Solve the given initial value problem:

⑤ $\frac{d^2y}{dx^2} - 4\frac{dy}{dx} - 5y = 0$; $y(1) = 0$; $y'(1) = 2$

\uparrow \uparrow \uparrow
 x y x y'

$$y'' - 4y' - 5y = 0 \quad \text{--- (i)}$$

Substitute $y = e^{mx}$, $y' = me^{mx}$, $y'' = m^2 e^{mx}$ into (i)

$$m^2 e^{mx} - 4me^{mx} - 5e^{mx} = 0 \quad (\div \text{ by } e^{mx})$$

$$m^2 - 4m - 5 = 0$$

$$m^2 - 5m + m - 5 = 0$$

$$(m-5)(m+1) = 0 \Rightarrow m_1 = 5, m_2 = -1$$

$$\therefore y = c_1 e^{5x} + c_2 e^{-x} \quad \text{--- (ii)}$$

$$y(1) = c_1 e^{5(1)} + c_2 e^{-1}$$

$$y(1) = c_1 e^5 + c_2 \frac{1}{e} \quad \text{--- (a)}$$

$$(a) + (b) \Rightarrow 6c_1 e^5 = 2$$

$$c_1 = \frac{1}{3e^5}$$

Substitute c_1 & c_2 into (ii)

$$y = \frac{1}{3e^5} \cdot e^{5x} - \frac{e}{3} \cdot e^{-x}$$

$$= \frac{1}{3} [e^{5(x-1)} - e^{(1-x)}]$$

$$y' = 5c_1 e^{5x} - c_2 e^{-x}$$

$$y'(1) = 5c_1 e^{5(1)} - c_2 e^{-1}$$

$$2 = 5c_1 e^5 - c_2 \frac{1}{e} \quad \text{--- (b)}$$

Substitute c_1 into (a)

$$\frac{1}{3e^5} \cdot e^5 + c_2 \frac{1}{e} = 0$$

$$\frac{1}{3} + c_2 \frac{1}{e} = 0$$

$$\frac{c_2}{e} = -\frac{1}{3} \Rightarrow c_2 = -\frac{e}{3}$$